proof/garble/equivFake.ec
@@ -1,6 +1,7 @@
 require import Bitstring.
 require import List.
 require import Map.
+import PartialGet.
 require import Set.
 require import Pair.
 require import Real.
@@ -18,6 +19,7 @@ module Fake(A:Garble.Adv) = {
 
   var f1 : Garble.funct
   var x1 : Garble.input
+  var ev : Garble.output
   var good : bool
   var tau : bool
   var queries : DKC.query array
@@ -32,7 +34,6 @@ module Fake(A:Garble.Adv) = {
   var bb : w2g
   var pp : token g2v
   var t : bool array
-  var v : bool array
   var xx : tokens
   var randG : (int*bool*bool, token) map
   var a : int
@@ -53,6 +54,7 @@ module Fake(A:Garble.Adv) = {
     var output : int*bool;
     var ra : bool;
     var ki : token;
+    var ko : token;
     var tok : token;
     var zz : token;
 
@@ -62,14 +64,21 @@ module Fake(A:Garble.Adv) = {
       ra = $Dbool.dbool;
       output = (g + n + q, ra);
     } else
-      output = (g, true (*TODO (evalGate gg.[g] ((v.[a]^^alpha),(v.[b]^^bet)))*));
+      output = (g, t.[g]);
 
 
 
     (*DKC encrypt*)
         tok = $DKC.genRandKey;
-        ki = proj kpub.[input];
-        zz = DKC.encode ttt (proj kpub.[input]) ksec tok;
+          
+        if (! (in_dom input DKC.Dkc.kpub)) {DKC.Dkc.kpub.[input] = $DKC.genRandKeyLast; DKC.Dkc.kpub.[input] = DKC.addLast DKC.Dkc.kpub.[input] (snd input);}
+        if (! (in_dom output DKC.Dkc.kpub)) {DKC.Dkc.kpub.[output] = $DKC.genRandKeyLast; DKC.Dkc.kpub.[output] = DKC.addLast DKC.Dkc.kpub.[output] (snd output);}
+        if (! (in_dom output DKC.Dkc.r)) DKC.Dkc.r.[output] = $DKC.genRandKey;
+
+        tok = r.[output];
+        ki = kpub.[input];
+        ko = kpub.[output];
+        zz = DKC.encode ttt ki ksec tok;
     (*End DKC encrypt*)
      
 
@@ -80,20 +89,22 @@ module Fake(A:Garble.Adv) = {
 
     ans = sub ans 0 ((length ans) - 1);
     pp.[g] = setGateVal pp.[g] ((t.[a]^^alpha), (t.[b]^^bet)) zz;
-    xx = setTok xx g (v.[a]^^alpha) ki;
+    xx = setTok xx g alpha ki;
+    if (!rand)
+      xx = setTok xx g false ko;
   }
 
   fun garb(yy:token, alpha:bool, bet:bool) : unit = {
     pp.[g] = setGateVal pp.[g] ((t.[a]^^alpha), (t.[b]^^bet)) (DKC.encode
       (tweak g (t.[a]^^alpha) (t.[b]^^bet))
-      (getTok xx a (v.[a]^^alpha))
-      (getTok xx b (v.[b]^^alpha))
+      (getTok xx a alpha)
+      (getTok xx b bet)
       yy);
   }
 
   fun garbD(alpha:bool, bet:bool) : token = {
     var yy : token;
-    yy = proj randG.[(g,alpha,bet)];
+    yy = randG.[(g,alpha,bet)];
     garb(yy, alpha, bet);
     return yy;
   }
@@ -109,12 +120,10 @@ module Fake(A:Garble.Adv) = {
 
     i = 0;
     while (i < n+q-m) {
-      v.[i] = eval f1 x1 i;
       t.[i] = $Dbool.dbool;
       i = i + 1;
     }
     while (i < n+q) {
-      v.[i] = eval f1 x1 i;
       t.[i] = false;
       i = i + 1;
     }
@@ -131,20 +140,22 @@ module Fake(A:Garble.Adv) = {
         query(true, true, true);
         preGarbD(true, false);
       } else {
-        preGarbD(true, false);
         preGarbD(false, true);
         preGarbD(true, true);
+        preGarbD(true, false);
       }
       g = g + 1;
     }
 
     i = 0;
     while (i < n+q) {
-      tok = $DKC.genRandKeyLast (! t.[i]);
-      if (getTok xx i true = void /\ i <> 0) {
+      tok = $DKC.genRandKeyLast;
+      tok = DKC.addLast tok (! t.[i]);
+      if (getTok xx i true = void /\ i <> bound - 1) {
         xx = setTok xx i true tok;
       }
-      tok = $DKC.genRandKeyLast (t.[i]);
+      tok = $DKC.genRandKeyLast;
+      tok = DKC.addLast tok (t.[i]);
       if (getTok xx i false = void) {
         xx = setTok xx i false tok;
       }
@@ -155,7 +166,7 @@ module Fake(A:Garble.Adv) = {
     while (g < n+q) {
       a = aa.[g];
       b = bb.[g];
-      garb(getTok xx g v.[g], false, false);
+      garb(getTok xx g false, false, false);
       if (b <> bound - 1) {
         tok = garbD(false, true);
         tok = garbD(true, true);
@@ -165,7 +176,7 @@ module Fake(A:Garble.Adv) = {
       }
       g = g + 1;
     }
-    answer = ((getN f1, getM f1, getQ f1, getA f1, getB f1, pp), encrypt (Array.sub xx 0 (getN f1)) x1,tt);
+    answer = ((getN f1, getM f1, getQ f1, getA f1, getB f1, pp), encrypt (Array.sub xx 0 (getN f1)) (Array.init (getN f1) false),tt);
   }
 
   fun work() : bool = {
@@ -179,15 +190,16 @@ module Fake(A:Garble.Adv) = {
     if (Garble.queryValid query)
     {
       tau = $Dbool.dbool;
-      ksec = $DKC.genRandKeyLast tau;
+      ksec = $DKC.genRandKeyLast;
+      ksec = DKC.addLast ksec tau;
       kpub = Map.empty;
       r = Map.empty;
 
       (f1, x1) = fst query;
       (n, m, q, aa, bb, gg) = f1;
+      ev = Garble.eval f1 x1;
       queries = Array.empty;
       t = Array.init (n+q) false;
-      v = Array.init (n+q) false;
       xx = Array.init (n+q) (void, void);
       pp = Array.init (n+q) (void, void, void, void);
       randG = Map.empty;
@@ -203,6 +215,31 @@ module Fake(A:Garble.Adv) = {
 
 }.
 
+prover "Alt-Ergo".
+
+lemma fakePr :
+  forall (ADV <: Garble.Adv{AdvAda, DKC.Dkc, Fake}) &m,
+    islossless ADV.gen_query =>
+    islossless ADV.get_challenge =>
+    Pr [Fake(ADV).work() @ &m : res] = 1%r / 2%r.
+intros ADV &m h1 h2.
+bdhoare_deno (_ : (true) ==> (res));last 2 by progress.
+fun.
+seq 1 : (true).
+call (_ : true ==> true);[fun (true)|skip];progress;assumption.
+case (queryValid Fake.query).
+  (* VALID *)
+  rcondt 1;first skip;progress.
+  wp.
+  rnd (1%r/2%r) (lambda b, (b = challenge) = false).
+  call (_ : true ==> true);first fun (true);progress;assumption.
+  kill 1!14;first admit. (*TERMINATE*)
+  skip;progress;rewrite Dbool.mu_def;case (result);delta charfun;simplify;smt.
+  (* INVALID *)
+  rcondf 1;first skip;progress.
+  rnd (1%r/2%r) (lambda b, b = false).
+  skip;progress;smt "Z3".
+save.
 
 lemma fakeEq :
   forall (ADV <: Garble.Adv{AdvAda, DKC.Dkc, Fake}),
@@ -233,32 +270,37 @@ proof strict.
   inline {2} Fake(ADV).garb.
   inline {2} Fake(ADV).preGarbD.
 
-  swap{1} 8 -7.
+  swap{1} 9 -8.
 
   seq 1 1 : ((glob ADV){1} = (glob ADV){2}/\AdvAda.query{1} = Fake.query{2} /\ (!DKC.Dkc.b{1}) /\ (AdvAda.l{1}=bound-1)).
-    call ((glob ADV){1} = (glob ADV){2}) (res{1}=res{2} /\ (glob ADV){1} = (glob ADV){2});first (fun true;by progress).
+    call (_ : (glob ADV){1} = (glob ADV){2} ==> res{1}=res{2} /\ (glob ADV){1} = (glob ADV){2});first (fun true;by progress).
   skip;progress;assumption.
   
   case (Garble.queryValid Fake.query{2}).
 
   (*VALID*)
-  rcondt {1} 19;first (intros _;wp;rnd;wp;rnd;rnd;skip;progress assumption).
+  rcondt {1} 20;first (intros _;wp;rnd;wp;rnd;rnd;skip;progress assumption).
   rcondt {2} 1;first (intros &m;skip;by progress).
 
-  swap{1} 8 -7.
-  swap{2} 25 -24.
+  swap{1} 9 -8.
+  swap{2} 26 -25.
 
   wp.
-  call ((glob ADV){1} = (glob ADV){2}/\answer{1}=answer{2}) (res{1}=res{2});first (fun true;by progress).
+  call (_ : (glob ADV){1} = (glob ADV){2}/\answer{1}=answer{2} ==> res{1}=res{2});first (fun true;by progress).
   wp.
+
+(*
+       (forall i, i>= 0 => i < Fake.n{2} => AdvAda.v{1}.[i] = AdvAda.xc{1}.[i]) /\
+       (forall i, i>= 0 => i < Fake.n{2} => Fake.v{2}.[i] = Fake.x1{2}.[i]) /\
+*)
 
   while (
+      Fake.ev{2} = Garble.eval AdvAda.fc{1} AdvAda.xc{1} /\
       (glob ADV){1} = (glob ADV){2} /\
       length AdvAda.xx{1} = AdvAda.n{1}+AdvAda.q{1} /\
       length AdvAda.t{1} = AdvAda.n{1}+AdvAda.q{1} /\
-      AdvAda.xx{1} = Fake.xx{2} /\
+      AdvAda.xx{1} = Fake.xx{2}/\
       AdvAda.t{1} = Fake.t{2}/\
-      AdvAda.v{1} = Fake.v{2}/\
       AdvAda.n{1} = Fake.n{2}/\
       AdvAda.m{1} = Fake.m{2}/\
       AdvAda.q{1} = Fake.q{2}/\
@@ -266,31 +308,30 @@ proof strict.
       AdvAda.bb{1} = Fake.bb{2}/\
       AdvAda.randG{1} = Fake.randG{2}/\
       AdvAda.pp{1} = Fake.pp{2}/\
-      AdvAda.fc{1} = Fake.f1{2}/\
-      AdvAda.xc{1} = Fake.x1{2}/\
       Fake.n{2} > 1/\
       Fake.m{2} > 0/\
       Fake.q{2} > 0/\
       (*Fake.f1{2} = (Fake.n{2}, Fake.m{2}, Fake.q{2}, Fake.aa{2}, Fake.bb{2}, Fake.gg{2}) /\*)
       Fake.n{2} + Fake.q{2} - Fake.m{2} = bound /\
       AdvAda.l{1} = bound-1 /\
-    (forall i, i >= Fake.n{2} => i < Fake.n{2}+Fake.q{2} => Fake.aa{2}.[i] >= 0 /\
-           Fake.bb{2}.[i] < bound /\ Fake.bb{2}.[i] < i /\ Fake.aa{2}.[i] < Fake.bb{2}.[i]) /\
-    (forall g, if (AdvAda.bb{1}.[g] = bound-1 /\ evalGate AdvAda.gg{1}.[g]
-      ((!AdvAda.v{1}.[AdvAda.aa{1}.[g]]), false) = evalGate AdvAda.gg{1}.[g] ((!AdvAda.v{1}.[AdvAda.aa{1}.[g]]), true)) then
-        AdvAda.yy{1}.[g]=proj Fake.randG{2}.[(g, true, false)] else true)/\
+    (forall i, i >= Fake.n{2} => i < Fake.n{2}+Fake.q{2} => Fake.aa{2}.[i] >= 0 /\ Fake.bb{2}.[i] < i /\
+           Fake.bb{2}.[i] < bound /\ Fake.aa{2}.[i] < Fake.bb{2}.[i]) /\
+    (forall g, g >= Fake.n{2} => g < Fake.n{2}+Fake.q{2} => AdvAda.bb{1}.[g] = bound-1 /\ evalGate AdvAda.gg{1}.[g]
+      ((!AdvAda.v{1}.[AdvAda.aa{1}.[g]]), false) = evalGate AdvAda.gg{1}.[g] ((!AdvAda.v{1}.[AdvAda.aa{1}.[g]]), true) =>
+        AdvAda.yy{1}.[g]=Fake.randG{2}.[(g, true, false)])/\
 
     AdvAda.g{1} = Fake.g{2} /\
       Fake.g{2} >= Fake.n{2} /\
     true
   ).
+
     seq 6 6 : (
+      Fake.ev{2} = Garble.eval AdvAda.fc{1} AdvAda.xc{1} /\
       (glob ADV){1} = (glob ADV){2} /\
       length AdvAda.xx{1} = AdvAda.n{1}+AdvAda.q{1} /\
       length AdvAda.t{1} = AdvAda.n{1}+AdvAda.q{1} /\
-      AdvAda.xx{1} = Fake.xx{2} /\
+      AdvAda.xx{1} = Fake.xx{2}/\
       AdvAda.t{1} = Fake.t{2}/\
-      AdvAda.v{1} = Fake.v{2}/\
       AdvAda.n{1} = Fake.n{2}/\
       AdvAda.m{1} = Fake.m{2}/\
       AdvAda.q{1} = Fake.q{2}/\
@@ -298,33 +339,32 @@ proof strict.
       AdvAda.bb{1} = Fake.bb{2}/\
       AdvAda.randG{1} = Fake.randG{2}/\
       AdvAda.pp{1} = Fake.pp{2}/\
-      AdvAda.fc{1} = Fake.f1{2}/\
-      AdvAda.xc{1} = Fake.x1{2}/\
       Fake.n{2} > 1/\
       Fake.m{2} > 0/\
       Fake.q{2} > 0/\
       (*Fake.f1{2} = (Fake.n{2}, Fake.m{2}, Fake.q{2}, Fake.aa{2}, Fake.bb{2}, Fake.gg{2}) /\*)
       Fake.n{2} + Fake.q{2} - Fake.m{2} = bound /\
       AdvAda.l{1} = bound-1 /\
-    (forall i, i >= Fake.n{2} => i < Fake.n{2}+Fake.q{2} => Fake.aa{2}.[i] >= 0 /\
-           Fake.bb{2}.[i] < bound /\ Fake.bb{2}.[i] < i /\ Fake.aa{2}.[i] < Fake.bb{2}.[i]) /\
-    (forall g, if (AdvAda.bb{1}.[g] = bound-1 /\ evalGate AdvAda.gg{1}.[g]
-      ((!AdvAda.v{1}.[AdvAda.aa{1}.[g]]), false) = evalGate AdvAda.gg{1}.[g] ((!AdvAda.v{1}.[AdvAda.aa{1}.[g]]), true)) then
-        AdvAda.yy{1}.[g]=proj Fake.randG{2}.[(g, true, false)] else true)/\
+    (forall i, i >= Fake.n{2} => i < Fake.n{2}+Fake.q{2} => Fake.aa{2}.[i] >= 0 /\ Fake.bb{2}.[i] < i /\
+           Fake.bb{2}.[i] < bound /\ Fake.aa{2}.[i] < Fake.bb{2}.[i]) /\
+    (forall g, g >= Fake.n{2} => g < Fake.n{2}+Fake.q{2} => AdvAda.bb{1}.[g] = bound-1 /\ evalGate AdvAda.gg{1}.[g]
+      ((!AdvAda.v{1}.[AdvAda.aa{1}.[g]]), false) = evalGate AdvAda.gg{1}.[g] ((!AdvAda.v{1}.[AdvAda.aa{1}.[g]]), true) =>
+        AdvAda.yy{1}.[g]=Fake.randG{2}.[(g, true, false)])/\
 
 
-    (if (AdvAda.b{1} = bound-1 /\ evalGate AdvAda.gg{1}.[Fake.g{2}]
-      ((!AdvAda.v{1}.[AdvAda.a{1}]), false) = evalGate AdvAda.gg{1}.[Fake.g{2}] ((!AdvAda.v{1}.[AdvAda.a{1}]), true)) then
-        AdvAda.yy{1}.[Fake.g{2}]=proj Fake.randG{2}.[(Fake.g{2}, true, false)] else true)/\
+    (AdvAda.b{1} = bound-1 /\ evalGate AdvAda.gg{1}.[Fake.g{2}]
+      ((!AdvAda.v{1}.[AdvAda.a{1}]), false) = evalGate AdvAda.gg{1}.[Fake.g{2}] ((!AdvAda.v{1}.[AdvAda.a{1}]), true) =>
+        AdvAda.yy{1}.[Fake.g{2}]=Fake.randG{2}.[(Fake.g{2}, true, false)])/\
       AdvAda.g{1} = Fake.g{2} /\
       Fake.g{2} >= Fake.n{2} /\
       AdvAda.a{1} = Fake.a{2} /\
       AdvAda.b{1} = Fake.b{2} /\
+      Fake.a{2} >= 0 /\
+      Fake.b{2} >= 0 /\
       AdvAda.a{1} < bound-1 /\
       AdvAda.b{1} <= bound-1 /\
       true
-    );first wp;skip;(progress assumption;first apply H6;progress;assumption);smt.
-
+    );first wp;skip;(progress assumption;first apply H6);smt.
     if;first smt.
       (*IF TRUE*)
       rcondt{1} 4;first (intros _;wp;skip;smt).
@@ -335,20 +375,17 @@ proof strict.
       (*IF FALSE*)
       rcondf{1} 1;first (intros _;skip;smt).
       cfold{1} 1?1.
-      (wp;skip;progress assumption;first rewrite H7);smt.
-  
+      wp;skip;progress assumption;smt.
 
   wp.
 
-
-
   while (
+      Fake.ev{2} = Garble.eval AdvAda.fc{1} AdvAda.xc{1} /\
       (glob ADV){1} = (glob ADV){2} /\
       length AdvAda.xx{1} = AdvAda.n{1}+AdvAda.q{1} /\
       length AdvAda.t{1} = AdvAda.n{1}+AdvAda.q{1} /\
-      AdvAda.xx{1} = Fake.xx{2} /\
+      AdvAda.xx{1} = Fake.xx{2}/\
       AdvAda.t{1} = Fake.t{2}/\
-      AdvAda.v{1} = Fake.v{2}/\
       AdvAda.n{1} = Fake.n{2}/\
       AdvAda.m{1} = Fake.m{2}/\
       AdvAda.q{1} = Fake.q{2}/\
@@ -356,42 +393,34 @@ proof strict.
       AdvAda.bb{1} = Fake.bb{2}/\
       AdvAda.randG{1} = Fake.randG{2}/\
       AdvAda.pp{1} = Fake.pp{2}/\
-      AdvAda.fc{1} = Fake.f1{2}/\
-      AdvAda.xc{1} = Fake.x1{2}/\
       Fake.n{2} > 1/\
       Fake.m{2} > 0/\
       Fake.q{2} > 0/\
       (*Fake.f1{2} = (Fake.n{2}, Fake.m{2}, Fake.q{2}, Fake.aa{2}, Fake.bb{2}, Fake.gg{2}) /\*)
       Fake.n{2} + Fake.q{2} - Fake.m{2} = bound /\
       AdvAda.l{1} = bound-1 /\
-    (forall i, i >= Fake.n{2} => i < Fake.n{2}+Fake.q{2} => Fake.aa{2}.[i] >= 0 /\
-           Fake.bb{2}.[i] < bound /\ Fake.bb{2}.[i] < i /\ Fake.aa{2}.[i] < Fake.bb{2}.[i]) /\
-    (forall g, if (AdvAda.bb{1}.[g] = bound-1 /\ evalGate AdvAda.gg{1}.[g]
-      ((!AdvAda.v{1}.[AdvAda.aa{1}.[g]]), false) = evalGate AdvAda.gg{1}.[g] ((!AdvAda.v{1}.[AdvAda.aa{1}.[g]]), true)) then
-        AdvAda.yy{1}.[g]=proj Fake.randG{2}.[(g, true, false)] else true)/\
+    (forall i, i >= Fake.n{2} => i < Fake.n{2}+Fake.q{2} => Fake.aa{2}.[i] >= 0 /\ Fake.bb{2}.[i] < i /\
+           Fake.bb{2}.[i] < bound /\ Fake.aa{2}.[i] < Fake.bb{2}.[i]) /\
+    (forall g, g >= Fake.n{2} => g < Fake.n{2}+Fake.q{2} => AdvAda.bb{1}.[g] = bound-1 /\ evalGate AdvAda.gg{1}.[g]
+      ((!AdvAda.v{1}.[AdvAda.aa{1}.[g]]), false) = evalGate AdvAda.gg{1}.[g] ((!AdvAda.v{1}.[AdvAda.aa{1}.[g]]), true) =>
+        AdvAda.yy{1}.[g]=Fake.randG{2}.[(g, true, false)])/\
 
     AdvAda.i{1} = Fake.i{2} /\
       0 <= Fake.i{2} /\
     true
   ).
-  wp.
-  rnd.
-  wp.
-  rnd.
-  skip.
-  progress assumption;last 4 smt.
-    delta setTok;simplify;rewrite ! set_length;try assumption;smt.
-    smt.
-    delta setTok;simplify;rewrite ! set_length;try assumption;smt.
+  wp;rnd;wp;rnd;skip.
+  progress assumption;smt.
+
   wp.
 
   while (
+      Fake.ev{2} = Garble.eval AdvAda.fc{1} AdvAda.xc{1} /\
       (glob ADV){1} = (glob ADV){2} /\
       length AdvAda.xx{1} = AdvAda.n{1}+AdvAda.q{1} /\
       length AdvAda.t{1} = AdvAda.n{1}+AdvAda.q{1} /\
-      AdvAda.xx{1} = Fake.xx{2} /\
+      AdvAda.xx{1} = Fake.xx{2}/\
       AdvAda.t{1} = Fake.t{2}/\
-      AdvAda.v{1} = Fake.v{2}/\
       AdvAda.n{1} = Fake.n{2}/\
       AdvAda.m{1} = Fake.m{2}/\
       AdvAda.q{1} = Fake.q{2}/\
@@ -399,35 +428,31 @@ proof strict.
       AdvAda.bb{1} = Fake.bb{2}/\
       AdvAda.randG{1} = Fake.randG{2}/\
       AdvAda.pp{1} = Fake.pp{2}/\
-      AdvAda.fc{1} = Fake.f1{2}/\
-      (AdvAda.c{1} = DKC.Dkc.b{1}) = PrvInd.b{2}/\
-      AdvAda.xc{1} = Fake.x1{2}/\
       Fake.n{2} > 1/\
       Fake.m{2} > 0/\
       Fake.q{2} > 0/\
       (*Fake.f1{2} = (Fake.n{2}, Fake.m{2}, Fake.q{2}, Fake.aa{2}, Fake.bb{2}, Fake.gg{2}) /\*)
       Fake.n{2} + Fake.q{2} - Fake.m{2} = bound /\
       AdvAda.l{1} = bound-1 /\
-    (forall i, i >= Fake.n{2} => i < Fake.n{2}+Fake.q{2} => Fake.aa{2}.[i] >= 0 /\
-           Fake.bb{2}.[i] < bound /\ Fake.bb{2}.[i] < i /\ Fake.aa{2}.[i] < Fake.bb{2}.[i]) /\
-    (forall g, if (AdvAda.bb{1}.[g] = bound-1 /\ evalGate AdvAda.gg{1}.[g]
-      ((!AdvAda.v{1}.[AdvAda.aa{1}.[g]]), false) = evalGate AdvAda.gg{1}.[g] ((!AdvAda.v{1}.[AdvAda.aa{1}.[g]]), true)) then
-        AdvAda.yy{1}.[g]=proj Fake.randG{2}.[(g, true, false)] else true)/\
+    (forall i, i >= Fake.n{2} => i < Fake.n{2}+Fake.q{2} => Fake.aa{2}.[i] >= 0 /\ Fake.bb{2}.[i] < i /\
+           Fake.bb{2}.[i] < bound /\ Fake.aa{2}.[i] < Fake.bb{2}.[i]) /\
+    (forall g, g >= Fake.n{2} => g <= Fake.g{2} => AdvAda.bb{1}.[g] = bound-1 /\ evalGate AdvAda.gg{1}.[g]
+      ((!AdvAda.v{1}.[AdvAda.aa{1}.[g]]), false) = evalGate AdvAda.gg{1}.[g] ((!AdvAda.v{1}.[AdvAda.aa{1}.[g]]), true) =>
+        AdvAda.yy{1}.[g]=Fake.randG{2}.[(g, true, false)])/\
 
     AdvAda.g{1} = Fake.g{2} /\
       Fake.g{2} >= Fake.n{2} /\
+      (forall g a b, g >= Fake.g{2} => !(mem (tweak g a b) DKC.Dkc.used{1})) /\
     true
   ).
-    admit.
 
-  wp.
-  while (
+    seq 2 2 : (
+      Fake.ev{2} = Garble.eval AdvAda.fc{1} AdvAda.xc{1} /\
       (glob ADV){1} = (glob ADV){2} /\
       length AdvAda.xx{1} = AdvAda.n{1}+AdvAda.q{1} /\
       length AdvAda.t{1} = AdvAda.n{1}+AdvAda.q{1} /\
-      AdvAda.xx{1} = Fake.xx{2} /\
+      AdvAda.xx{1} = Fake.xx{2}/\
       AdvAda.t{1} = Fake.t{2}/\
-      AdvAda.v{1} = Fake.v{2}/\
       AdvAda.n{1} = Fake.n{2}/\
       AdvAda.m{1} = Fake.m{2}/\
       AdvAda.q{1} = Fake.q{2}/\
@@ -435,205 +460,188 @@ proof strict.
       AdvAda.bb{1} = Fake.bb{2}/\
       AdvAda.randG{1} = Fake.randG{2}/\
       AdvAda.pp{1} = Fake.pp{2}/\
-      AdvAda.fc{1} = Fake.f1{2}/\
-      AdvAda.xc{1} = Fake.x1{2}/\
       Fake.n{2} > 1/\
       Fake.m{2} > 0/\
       Fake.q{2} > 0/\
       (*Fake.f1{2} = (Fake.n{2}, Fake.m{2}, Fake.q{2}, Fake.aa{2}, Fake.bb{2}, Fake.gg{2}) /\*)
       Fake.n{2} + Fake.q{2} - Fake.m{2} = bound /\
       AdvAda.l{1} = bound-1 /\
-    (forall i, i >= Fake.n{2} => i < Fake.n{2}+Fake.q{2} => Fake.aa{2}.[i] >= 0 /\
-           Fake.bb{2}.[i] < bound /\ Fake.bb{2}.[i] < i /\ Fake.aa{2}.[i] < Fake.bb{2}.[i]) /\
+    (forall i, i >= Fake.n{2} => i < Fake.n{2}+Fake.q{2} => Fake.aa{2}.[i] >= 0 /\ Fake.bb{2}.[i] < i /\
+           Fake.bb{2}.[i] < bound /\ Fake.aa{2}.[i] < Fake.bb{2}.[i]) /\
+    (forall g, g >= Fake.n{2} => g <= Fake.g{2} => AdvAda.bb{1}.[g] = bound-1 /\ evalGate AdvAda.gg{1}.[g]
+      ((!AdvAda.v{1}.[AdvAda.aa{1}.[g]]), false) = evalGate AdvAda.gg{1}.[g] ((!AdvAda.v{1}.[AdvAda.aa{1}.[g]]), true) =>
+        AdvAda.yy{1}.[g]=Fake.randG{2}.[(g, true, false)])/\
+
+
+    (AdvAda.b{1} = bound-1 /\ evalGate AdvAda.gg{1}.[Fake.g{2}]
+      ((!AdvAda.v{1}.[AdvAda.a{1}]), false) = evalGate AdvAda.gg{1}.[Fake.g{2}] ((!AdvAda.v{1}.[AdvAda.a{1}]), true) =>
+        AdvAda.yy{1}.[Fake.g{2}]=Fake.randG{2}.[(Fake.g{2}, true, false)])/\
+      AdvAda.g{1} = Fake.g{2} /\
+      Fake.g{2} >= Fake.n{2} /\
+      AdvAda.a{1} = Fake.a{2} /\
+      AdvAda.b{1} = Fake.b{2} /\
+      Fake.a{2} >= 0 /\
+      Fake.b{2} >= 0 /\
+      AdvAda.a{1} < Fake.g{2} /\
+      AdvAda.b{1} < Fake.g{2} /\
+      AdvAda.a{1} < bound-1 /\
+      AdvAda.b{1} <= bound-1 /\
+      (forall g a b, g >= Fake.g{2} => !(mem (tweak g a b) DKC.Dkc.used{1})) /\
+      true
+    );first wp;skip;(progress assumption;first apply H6);smt.
+  rcondf{1} 1;first intros ?;wp;skip;progress assumption;smt.
+  if;first smt.
+
+  rcondf{1} 6;first intros ?;wp;skip;progress assumption;smt.
+  rcondt{1} 13;first intros ?;wp;rnd;wp;skip;progress assumption;smt.
+  rcondf{1} 23;first intros ?;(kill 1!22;first admit);skip;progress assumption;smt.
+  rcondt{1} 37;first intros ?;wp;rnd;wp;(kill 14!3;first admit);wp;rnd;wp;skip;
+    ((progress assumption;first 2 smt);first rewrite Set.add_mem;rewrite tweak_inj2);smt.
+  rcondf{1} 50;first intros ?;(kill 1!49;first admit);skip;by progress assumption.
+  rcondf{1} 50;first intros ?;(kill 1!49;first admit);skip;progress assumption;smt.
+  cfold{1} 50.
+  rcondt{1} 52;first intros ?;(kill 1!51;first admit);skip;progress assumption.
+  wp.
+  rnd.
+  wp.
+
+if.
+
+skip;progress assumption.
+(kill 8;first admit);wp;skip;progress assumption;smt.
+  wp.
+
+
+
+  wp.
+  while (
+      Fake.ev{2} = Garble.eval AdvAda.fc{1} AdvAda.xc{1} /\
+      (glob ADV){1} = (glob ADV){2} /\
+      length AdvAda.xx{1} = AdvAda.n{1}+AdvAda.q{1} /\
+      length AdvAda.t{1} = AdvAda.n{1}+AdvAda.q{1} /\
+      AdvAda.xx{1} = Fake.xx{2}/\
+      AdvAda.t{1} = Fake.t{2}/\
+      AdvAda.n{1} = Fake.n{2}/\
+      getN AdvAda.fc{1} = Fake.n{2}/\
+      AdvAda.m{1} = Fake.m{2}/\
+      getM AdvAda.fc{1} = Fake.m{2}/\
+      AdvAda.q{1} = Fake.q{2}/\
+      getQ AdvAda.fc{1} = Fake.q{2}/\
+      AdvAda.aa{1} = Fake.aa{2}/\
+      AdvAda.bb{1} = Fake.bb{2}/\
+      AdvAda.randG{1} = Fake.randG{2}/\
+      AdvAda.pp{1} = Fake.pp{2}/\
+      Fake.q{2} >= Fake.m{2}/\
+      Fake.n{2} > 1/\
+      Fake.m{2} > 0/\
+      Fake.q{2} > 0/\
+      (*Fake.f1{2} = (Fake.n{2}, Fake.m{2}, Fake.q{2}, Fake.aa{2}, Fake.bb{2}, Fake.gg{2}) /\*)
+      Fake.n{2} + Fake.q{2} - Fake.m{2} = bound /\
+      AdvAda.l{1} = bound-1 /\
+    (forall i, i >= Fake.n{2} => i < Fake.n{2}+Fake.q{2} => Fake.aa{2}.[i] >= 0 /\ Fake.bb{2}.[i] < i /\
+           Fake.bb{2}.[i] < bound /\ Fake.aa{2}.[i] < Fake.bb{2}.[i]) /\
 
     AdvAda.i{1} = Fake.i{2} /\
-      Fake.i{2} >= 0 /\
+      Fake.i{2} >= Fake.n{2} + Fake.q{2} - Fake.m{2} /\
     true
   );first (wp;skip;progress assumption;first (rewrite ! set_length;try assumption));smt.
 
   while (
+      Fake.ev{2} = Garble.eval AdvAda.fc{1} AdvAda.xc{1} /\
       (glob ADV){1} = (glob ADV){2} /\
       length AdvAda.xx{1} = AdvAda.n{1}+AdvAda.q{1} /\
       length AdvAda.t{1} = AdvAda.n{1}+AdvAda.q{1} /\
-      AdvAda.xx{1} = Fake.xx{2} /\
+      AdvAda.xx{1} = Fake.xx{2}/\
       AdvAda.t{1} = Fake.t{2}/\
-      AdvAda.v{1} = Fake.v{2}/\
       AdvAda.n{1} = Fake.n{2}/\
+      getN AdvAda.fc{1} = Fake.n{2}/\
       AdvAda.m{1} = Fake.m{2}/\
+      getM AdvAda.fc{1} = Fake.m{2}/\
       AdvAda.q{1} = Fake.q{2}/\
+      getQ AdvAda.fc{1} = Fake.q{2}/\
       AdvAda.aa{1} = Fake.aa{2}/\
       AdvAda.bb{1} = Fake.bb{2}/\
       AdvAda.randG{1} = Fake.randG{2}/\
       AdvAda.pp{1} = Fake.pp{2}/\
-      AdvAda.fc{1} = Fake.f1{2}/\
-      AdvAda.xc{1} = Fake.x1{2}/\
       Fake.n{2} > 1/\
       Fake.m{2} > 0/\
       Fake.q{2} > 0/\
       (*Fake.f1{2} = (Fake.n{2}, Fake.m{2}, Fake.q{2}, Fake.aa{2}, Fake.bb{2}, Fake.gg{2}) /\*)
       Fake.n{2} + Fake.q{2} - Fake.m{2} = bound /\
       AdvAda.l{1} = bound-1 /\
-    (forall i, i >= Fake.n{2} => i < Fake.n{2}+Fake.q{2} => Fake.aa{2}.[i] >= 0 /\
-           Fake.bb{2}.[i] < bound /\ Fake.bb{2}.[i] < i /\ Fake.aa{2}.[i] < Fake.bb{2}.[i]) /\
+    (forall i, i >= Fake.n{2} => i < Fake.n{2}+Fake.q{2} => Fake.aa{2}.[i] >= 0 /\ Fake.bb{2}.[i] < i /\
+           Fake.bb{2}.[i] < bound /\ Fake.aa{2}.[i] < Fake.bb{2}.[i]) /\
 
     AdvAda.i{1} = Fake.i{2} /\
       Fake.i{2} >= 0 /\
     true
-  );first (wp;rnd;wp;skip;progress assumption;first (rewrite ! set_length;try assumption));smt.
+  );first (
+  wp;
+  rnd;
+  wp;skip;progress assumption);smt.
 
 wp.
 swap 1 1.
-  wp;rnd;rnd;rnd.
-  skip.
+wp.
+rnd.
+rnd.
+rnd.
+skip.
 
 
   cut lem : (forall (x:int), x <= x);first smt.
   delta queryValid.
-  rewrite valid_wireinput.
+  delta phi.
+  rewrite ! valid_wireinput.
   delta fst snd getN getM getQ.
   intros &1 &2.
   elimT tuple2_ind Fake.query{2}.
-  intros query1 query2.
+  intros query1 query2 queryVal.
 
   elimT tuple2_ind query1.
-  intros f1 x1.
+  intros f1 x1 query1val.
   elimT tuple6_ind f1.
-  intros n1 m1 q1 aa1 bb1 gg1.
+  intros n1 m1 q1 aa1 bb1 gg1 f1val.
 
   elimT tuple2_ind query2.
-  intros f2 x2.
+  intros f2 x2 query2val.
   elimT tuple6_ind f2.
-  intros n2 m2 q2 aa2 bb2 gg2.
+  intros n2 m2 q2 aa2 bb2 gg2 f2val.
 
-(*Progress :
-  do ? (
-    do ? (
-      do ? (intros=> [hyp1 hyp2];generalize hyp1 hyp2);
-      intros ?
-    );
-    subst;simplify;
-    
-    do (try assumption;split);
-    try assumption
-  ).
-*)
-
-  do 2! (
-    do ? (
-      do ? (intros=> [hyp1 hyp2];generalize hyp1 hyp2);
-      intros ?
-    );
-    subst;simplify;
-    
-    do (try assumption;split);
-    try assumption
-  ).
   intros h.
 
-  La ligne suivant ne termine pas :
+    cut rew : (length x1 = length x2);first smt.
+    cut lem0 : (0 <= 0);first smt.
+    cut lem1 : (0 >= 0);first smt.
+    cut lem2 : (length x2 >= length x2);first smt.
+    cut lem3 : (length x2 >= 1);first smt.
+    cut lem4 : (0 <= length x2 + q2);first smt.
 
-  split.
+  generalize h.
 
+  generalize bound.
+  intros bound.
 
-    do ? (
-      do ? (intros=> [hyp1 hyp2];generalize hyp1 hyp2);
-      intros ?
-    ).
-    subst;simplify.
-    do (try assumption;split).
-    do intros ?.
-    split.
-    do intros ?.
-    assumption.
-    do ? (
-      do ? (intros=> [hyp1 hyp2];generalize hyp1 hyp2);
-      intros ?
-    ).
-    case cL.
-    do ? (
-      do ? (intros=> [hyp1 hyp2];generalize hyp1 hyp2);
-      intros ?
-    ).
-    split.
-    split.
-    apply init_length;smt.
-    split.
-    apply init_length;smt.
-    split.
-    assumption.
-    split.
-    assumption.
-    split.
-    assumption.
-    split.
-    assumption.
-    split.
-    assumption.
+  subst;simplify.
+  rewrite rew.
 
+  progress ((try rewrite rew);(try apply init_length);(try rewrite rew);assumption).
+  smt.
+  smt.
+  smt.
+  apply H48;smt.
   smt.
   smt.
   smt.
   smt.
-  smt.
-admit.
-admit.
-admit.
-admit.
-admit.
-admit.
-admit.
-admit.
-admit.
-  smt.
-  smt.
-  smt.
-  smt.
-  smt.
-  smt.
-  smt.
-  smt.
-  smt.
-  smt.
-  smt.
-  smt.
-  smt.
-  smt.
-  smt.
-  smt.
-  smt.
-  smt.
-  smt.
-  smt.
-  admit.
-  admit.
-  smt.
-  smt.
-  smt.
-  admit.
-  smt.
-  smt.
-  smt.
-  smt.
-  smt.
-  smt.
-  smt.
-  smt.
-  smt.
-  smt.
-  smt.
-  smt.
-  smt.
-  smt.
-  smt.
-  smt.
-  smt.
+  apply H51;smt.
   smt.
 
   (*INVALID*)
-  rcondf {1} 18;first (intros _;wp;rnd;wp;rnd;rnd;skip;smt).
+  rcondf {1} 20;first (intros _;wp;rnd;wp;rnd;rnd;skip;smt).
   rcondf {2} 1;[intros &m;skip;smt|].
   wp.
-  kill{1} 1!17;first (wp;rnd 1%r cPtrue;wp;rnd 1%r cPtrue;rnd 1%r cPtrue;skip;progress;smt).
+  kill{1} 1!19;first (wp;rnd 1%r cpTrue;wp;rnd 1%r cpTrue;rnd 1%r cpTrue;skip;progress;smt).
   rnd;skip;progress assumption;smt.
 
 save.
